Proved distinct is decidable

lean4/Automaton/DFA/Minimization.lean
@@ -80,6 +80,7 @@ lemma distinct_if_δ_star'_distinct (w : word t.σs) : (a b : t.qs) → distinct
                 apply distinct.step
                 exact d
 
+
 theorem distinct_iff_ex_notaccepted (a b : t.qs) : distinct t a b ↔ ∃ l : word t.σs, ¬(δ_star' t a l ∈ t.fs ↔ δ_star' t b l ∈ t.fs) := by
   apply Iff.intro
   · intro d
@@ -155,25 +156,23 @@ instance instNondistinctEquivalence : Equivalence (nondistinct t) := by
   · exact nondistinct.Symm t
   · exact nondistinct.Trans t
 
+-- Table filling algorithm
+
 def all_pairs : Finset (t.qs × t.qs) := t.qs.attach.biUnion (fun q₁ => t.qs.attach.biUnion (fun q₂ => {⟨q₁,q₂⟩}))
 
 def start : Finset (t.qs × t.qs) := (all_pairs t).filter (fun (a,b) => ¬(a ∈ t.fs ↔ b ∈ t.fs))
 
-def step (c a : Finset (t.qs × t.qs)) : Finset (t.qs × t.qs) :=  c ∪ (a.filter (fun (a,b) => ∃ s : t.σs, (t.δ a s, t.δ b s) ∈ c))
+lemma start_subset_all : (start t) ⊆ (all_pairs t) := by
+  simp [start]
 
-def aux (c : Finset (t.qs × t.qs)) (h : c ⊆ (all_pairs t)) : Finset (t.qs × t.qs) := by
-  let a := all_pairs t
-  if g : (step t c a).card = c.card then exact c else exact aux (step t c a) (by simp only [step]
-                                                                                 apply Finset.union_subset_iff.mpr
-                                                                                 apply And.intro
-                                                                                 · exact h
-                                                                                 · simp)
+def step (c a : Finset (t.qs × t.qs)) : Finset (t.qs × t.qs) := c ∪ (a.filter (fun (a,b) => ∃ s : t.σs, (t.δ a s, t.δ b s) ∈ c))
 
-termination_by aux c h => (all_pairs t).card - c.card
-decreasing_by have h₁ : (step t c a).card >= c.card := by simp only [step]
+theorem table_aux_decreasing : ¬card (step t c (all_pairs t)) = card c → c ⊆ all_pairs t → (all_pairs t).card - (step t c (all_pairs t)).card < (all_pairs t).card - c.card := by
+  intro g h
+  have h₁ : (step t c (all_pairs t)).card >= c.card := by simp only [step]
                                                           apply Finset.card_le_of_subset
                                                           apply Finset.subset_union_left
-              have h₂ : card c < card (step t c a) := by apply Nat.lt_iff_le_and_ne.mpr
+  have h₂ : card c < card (step t c (all_pairs t)) := by apply Nat.lt_iff_le_and_ne.mpr
                                                          apply And.intro
                                                          · exact h₁
                                                          · simp at g
@@ -182,37 +181,179 @@ decreasing_by have h₁ : (step t c a).card >= c.card := by simp only [step]
                                                            simp at eq
                                                            apply Eq.symm
                                                            exact eq
-              have s : step t c a ⊆ a := by simp only [step]
-                                            apply Finset.union_subset
-                                            · exact h
-                                            · apply Finset.filter_subset
-              have d : c ⊂ step t c a := by apply Finset.ssubset_iff_subset_ne.mpr
+  have s : step t c (all_pairs t) ⊆ (all_pairs t) := by simp only [step]
+                                                        apply Finset.union_subset
+                                                        · exact h
+                                                        · apply Finset.filter_subset
+  have d : c ⊂ step t c (all_pairs t) := by apply Finset.ssubset_iff_subset_ne.mpr
                                             apply And.intro
                                             · simp only [step]
                                               apply Finset.subset_union_left
                                             · intro eq
                                               apply g
                                               rw [←eq]
-              have : a.card - (step t c a).card < a.card - c.card := by apply Nat.sub_lt_sub_left
-                                                                        · apply Nat.lt_iff_le_and_ne.mpr
-                                                                          apply And.intro
-                                                                          · apply Finset.card_le_of_subset
-                                                                            exact h
-                                                                          · apply Nat.ne_of_lt
-                                                                            apply Finset.card_lt_card
-                                                                            apply Finset.ssubset_of_ssubset_of_subset
-                                                                            · exact d
-                                                                            · exact s
-                                                                        · exact h₂
+  have : (all_pairs t).card - (step t c (all_pairs t)).card < (all_pairs t).card - c.card := by apply Nat.sub_lt_sub_left
+                                                                                                · apply Nat.lt_iff_le_and_ne.mpr
+                                                                                                  apply And.intro
+                                                                                                  · apply Finset.card_le_of_subset
+                                                                                                    exact h
+                                                                                                  · apply Nat.ne_of_lt
+                                                                                                    apply Finset.card_lt_card
+                                                                                                    apply Finset.ssubset_of_ssubset_of_subset
+                                                                                                    · exact d
+                                                                                                    · exact s
+                                                                                                · exact h₂
+  exact this
+
+def table_aux (c : Finset (t.qs × t.qs)) (h : c ⊆ (all_pairs t)) : Finset (t.qs × t.qs) := by
+  let a := all_pairs t
+  if (step t c a).card = c.card then exact c else exact table_aux (step t c a) (by simp only [step]
+                                                                                   apply Finset.union_subset_iff.mpr
+                                                                                   apply And.intro
+                                                                                   · exact h
+                                                                                   · simp)
+termination_by table_aux c h => (all_pairs t).card - c.card
+decreasing_by have : (all_pairs t).card - (step t c (all_pairs t)).card < (all_pairs t).card - c.card := by apply table_aux_decreasing t (by assumption) (by assumption)
               apply this
 
-
-
-lemma start_subset_all : (start t) ⊆ (all_pairs t) := by
-  simp [start]
-
-def table_filling : Finset (t.qs × t.qs) := aux t (start t) (start_subset_all t)
+def table_filling : Finset (t.qs × t.qs) := table_aux t (start t) (start_subset_all t)
 
 def distinct_table_filling (a b : t.qs) : Bool := ⟨a,b⟩ ∈ table_filling t
 
-instance : Decidable (distinct t a b) := sorry
+lemma step_subset (a b : Finset _) : a ⊆ b → step t a b ⊆ b := by
+  intro ss
+  simp only [step]
+  apply Finset.union_subset_iff.mpr
+  apply And.intro
+  · exact ss
+  · simp
+
+lemma table_aux_eq_table_aux : table_aux t c h = if (step t c (all_pairs t)).card = c.card then c else table_aux t (step t c (all_pairs t)) (step_subset t c (all_pairs t) h) := by
+  apply WellFounded.fixFEq
+
+theorem table_aux_forall (P : Finset (t.qs × t.qs) → Prop) (c : Finset (t.qs × t.qs)) {h : c ⊆ all_pairs t} : P c → (∀ f : Finset (t.qs × t.qs), P f → P (step t f (all_pairs t))) → P (table_aux t c h) := by
+  intro b fa
+  rw [table_aux_eq_table_aux]
+  split
+  · exact b
+  · apply table_aux_forall
+    · apply fa
+      exact b
+    · apply fa
+termination_by table_aux_forall p => (all_pairs t).card - c.card
+decreasing_by have : (all_pairs t).card - (step t c (all_pairs t)).card < (all_pairs t).card - c.card := by apply table_aux_decreasing t (by assumption) (by assumption)
+              apply this
+
+def ex_word_prop : Finset (t.qs × t.qs) → Prop := fun f => ∀ p : (t.qs × t.qs), p ∈ f → ∃ w : word t.σs, ¬(δ_star' t p.1 w ∈ t.fs ↔ δ_star' t p.2 w ∈ t.fs)
+
+lemma exists_notaccepted_if_table_filling : ex_word_prop t (table_aux t (start t) (start_subset_all t)) := by
+  apply table_aux_forall
+  · simp [ex_word_prop,start]
+    intro a b c d _ nin
+    exists []
+  · intro f p
+    simp [ex_word_prop] at p
+    simp [ex_word_prop,step]
+    intro a p₁ b p₂ h
+    cases h with
+    | inl h => apply p; exact h
+    | inr h => apply Exists.elim h.2
+               intro s h₁
+               apply Exists.elim h₁
+               intro p₃ e
+               have := p (t.δ ⟨a, p₁⟩ ⟨s , p₃⟩) (by simp) (t.δ ⟨b, p₂⟩ ⟨s , p₃⟩) (by simp) e
+               apply Exists.elim this
+               intro w h
+               rw [←distinct_iff_ex_notaccepted]
+               rw [←distinct_iff_ex_notaccepted] at this
+               apply distinct.step
+               exact this
+
+lemma step_gt_if (c : Finset _)(a b : t.qs) (e : t.σs): ⟨t.δ a e, t.δ b e⟩ ∈ c → ⟨a,b⟩ ∉ c → (step t c (all_pairs t)).card > c.card := by
+  intro inc ninc
+  simp only [step]
+  apply Finset.card_lt_card
+  have : c ⊆ c ∪ filter (fun x => ∃ s, (DFA.δ t x.fst s, DFA.δ t x.snd s) ∈ c) (all_pairs t) := by apply Finset.subset_union_left
+  have := Finset.ssubset_iff_of_subset this
+  apply this.mpr
+  exists ⟨a,b⟩
+  · apply And.intro
+    · apply Finset.mem_union_right
+      simp only [Finset.mem_filter]
+      apply And.intro
+      · simp [all_pairs]
+      · exists e
+    · exact ninc
+
+lemma if_δ_in_table_aux_in_table_aux : ⟨t.δ a e, t.δ b e⟩ ∈ table_aux t c h → ⟨a,b⟩ ∈ table_aux t c h := by
+  intro δ
+  rw [table_aux_eq_table_aux]
+  rw [table_aux_eq_table_aux] at δ
+  split
+  · split at δ
+    · cases (Decidable.em (⟨a,b⟩ ∈ c)) with
+      | inl h => exact h
+      | inr h => have := step_gt_if t c a b e δ h
+                 have : card (step t c (all_pairs t)) ≠ card c := by apply Nat.ne_of_gt
+                                                                     exact this
+                 contradiction
+    · contradiction
+  · split at δ
+    · contradiction
+    · apply if_δ_in_table_aux_in_table_aux
+      · exact δ
+termination_by if_δ_in_table_aux_in_table_aux p => (all_pairs t).card - c.card
+decreasing_by have : (all_pairs t).card - (step t c (all_pairs t)).card < (all_pairs t).card - c.card := by apply table_aux_decreasing t (by assumption) (by assumption)
+              apply this
+
+
+lemma table_filling_if_exists (w : word t.σs): (a b : t.qs) → ¬(δ_star' t a w ∈ t.fs ↔ δ_star' t b w ∈ t.fs) → distinct_table_filling t a b := by
+  simp only [distinct_table_filling,table_filling]
+  induction w  with
+  | nil => intro a b h
+           simp at h
+           rw [decide_eq_true_eq]
+           apply table_aux_forall
+           · simp [start]
+             simp at h
+             apply And.intro
+             · simp [all_pairs]
+             · exact h
+           · intro f inf
+             simp [step]
+             apply Or.inl
+             exact inf
+    | cons e es s => intro a b h
+                     rw [decide_eq_true_eq]
+                     simp at h
+                     have δ := s (t.δ a e) (t.δ b e) h
+                     rw [decide_eq_true_eq] at δ
+                     apply if_δ_in_table_aux_in_table_aux
+                     exact δ
+
+
+theorem forall_step_exists_word (a b : t.qs) : distinct_table_filling t a b ↔ ∃ w : word t.σs, ¬(δ_star' t a w ∈ t.fs ↔ δ_star' t b w ∈ t.fs) := by
+  apply Iff.intro
+  · intro d
+    simp only [distinct_table_filling] at d
+    rw [decide_eq_true_eq] at d
+    have := exists_notaccepted_if_table_filling t
+    simp only [ex_word_prop] at this
+    have := this ⟨a,b⟩
+    apply this
+    exact d
+  · intro ex
+    apply Exists.elim ex
+    intro w h
+    apply table_filling_if_exists
+    . exact h
+
+
+instance instDecExW : Decidable (∃ w : word t.σs, ¬(δ_star' t a w ∈ t.fs ↔ δ_star' t b w ∈ t.fs)) := by
+  apply decidable_of_iff (distinct_table_filling t a b)
+  exact forall_step_exists_word t a b
+
+instance instDecDistinct : Decidable (distinct t a b) := by
+  apply decidable_of_iff (∃ w : word t.σs, ¬(δ_star' t a w ∈ t.fs ↔ δ_star' t b w ∈ t.fs))
+  apply Iff.symm
+  apply distinct_iff_ex_notaccepted
